
FV(e) $\subseteq$ Empty cannot happen.


transitivty
sigma 1 -> sigma 2 -> sigma 3
sigma 1 -> sigma 3


$$
\dfrac{\sigma_1, (s_1;s_2)\Downarrow \sigma' s_3}{(\sigma_1, (s_1;s_2); s_3)}

$$


We just state for $\exists\ \sigma', \sigma''$ that $(\sigma_1, s_1) \Downarrow \sigma''$



do s until e $\equiv$ s; while $\neg e$ do s od





$$\dfrac{\dfrac{}{\{\varphi\}\ s\ \{\varphi\}}\quad\{\varphi\}\ while\ \neg e\ do\ s \ od\ \{\varphi\ \wedge\ e\}}{\{\varphi\}\ s;while\ \neg e\ do\ s \ od\ \{\varphi\ \wedge\ e\}}$$


$$
\{\varphi\}\ while\ \neg e\ do\ s \ od\ \{\varphi\ \wedge\ e\}
$$